RSA is in the category of asymmetric cryptography (public and private keys).
- uses a public key for encryption, and a private key for decnryption
- Anyone can encrypt, but only the owner can decrypt
## Key Generation
We want to generate two keys:
- public key $(e, n)$: used for encryption
- private key $(d,n)$: used for decryption
We do this through the following steps:
1. Choose two large prime numbers
	- Let $p$ and $q$ be distinct large primes
	- Then compute $n = p\cdot q$
2. Compute Euler's Totient Function
	- $\phi(n) = \phi(pq) = (p-1)(q-1)$ 
	- We do this because according to Euler's Theorem, 
		- If $\gcd(m,n) = 1$, then $m^{\phi(n)} \equiv 1 \mod n$ 
3. Choose a public exponent $e$
	- Pick an integer $e$ s.t.:
		- $1 < e < \phi(n)$
		- $\gcd(e, \phi(n)) = 1$ (ie. $e$ and $\phi(n)$ are coprime) 
4. Compute private exponent $d$
	- This is the modular inverse of $e$ modulo $\phi(n)$, meaning:
		- $d \cdot e \equiv 1 \mod \phi(n)$
	- This is computed using Reverse Euclidean Algorithm
At this point, we have:
- public key $(e,n)$
- private key (d, n)
## RSA Encryption
Suppose someone wants to send you a message $m \in \mathbb{Z}$. They do:
$$c = m^e \mod n$$
Where:
- $m$: original message (as an integer < n)
- $c$: ciphertext
- $e$: public exponent
- $n$: public modulus
## RSA Decryption
You, the owner of the private key, compute:
$$m = m^{e^d} = c^d \mod n$$
Because,
$$m^{ed} \equiv m \mod n$$
by Euler's Theorem, as long as $\gcd(m,n) = 1$

## Example
1. Choose two distinct primes
	- $p = 5$
	- $q = 11$
	- $n = pq = 5\cdot 11 = 55$
2. Compute Euler's Totient
	- $\phi(n) = \phi(55) = (p-1)(q-1) = (5-1)(11-1) = 40$
3. Choose a public exponent $e$
	- We need $1 < e < \phi(n) = 40$ s.t. $\gcd(e, 40) = 1$
	- Let's pick $e = 3$. $\gcd(3, 40) = 1$
4. Compute private exponent $d$
	- We want a $d$ s.t.:
		- $e \cdot d \equiv 1 \mod \phi(n)$ (ie. $d$ is the modular inverse of $e\mod \phi(n)$)
	- So we want:
		- $d \cdot e \equiv 1 \mod 40$
		- $d = 27$ (from extended EA)
Keys:
- public key: $(e,n) = (3,55)$
- private key: $(d,n) = (27,55)$

Suppose someone wants to send the message:
$$m = 12$$
To encrypt it using the public key $(e = 3, n = 55)$, they compute:
$$c = m^e \mod n = 12^e \mod 55 = 1728 \mod 55$$
$\Rightarrow c = 23$

You use your private key $(d = 27, n = 55)$ to decrypt:
$$m = c^d \mod n = 23^{27} \mod 55$$
You recover the original message $m = 12$.
## Proof / Rationale behind these steps
### Key Generation
#### Overall Goal
We want to construct a public key $(e,n)$ and a private key $(d,n)$ s.t.:
- **we first raise the message $m$ by $e$, send the ciphertext to the recipient, then raise that ciphertext again by $d$, and by $\mod n$, it returns back $m$.**
$$(m^e)^d \equiv m \mod n \Rightarrow m^{ed} \equiv m \mod n$$
#### Choose Two Large Primes $p$ and $q$, Compute $n$
We use the $p, q$ to form $n = pq$, which is the modulus for both encryption and decryption. 
<u>RSA Assumption</u>:The security of RSA relies on the assumption that it's hard to factor $n$ back into $p$ and $q$. 
Once someone knows $p$ and $q$, they can compute $\phi(n)$, and break RSA.
The reason we use two primes is that it **gives us a composite number $n$ whose totient is still easy to compute if you know the factors**.
#### Compute Euler's Totient (Proof)
We use the fact that $p,q$ are primes, so $$\phi(n) = \phi(pq) = (p-1)(q-1)$$
Euler's Theorem says that if $\gcd(m,n) = 1$, then $m^{\phi(n)}\equiv 1 \mod n$. This implies any multiple of $m^{\phi(n)}$ is equiv to 1 mod n, so 
$$m^{k\cdot \phi(n)} \equiv 1 \mod n$$
So if we choose $e, d$ s.t. 
$$ed \equiv 1 \mod \phi(n)$$
, implies 
$$ed = 1 + k\phi(n), \hspace{0.5em} k \in \mathbb{Z}$$
Substituting this into $m^{ed}$, 
$$m^{ed} = m^{1 + k\phi(n)} = m \cdot (m^{\phi(n)})^k$$
By Euler's Theorem:
$$m^{\phi(n)} \equiv 1 \mod n \Rightarrow (m^{\phi(n)})^k \equiv 1^k = 1 \mod n$$
So:
$$m^{ed} = m \cdot (m^{\phi(n)})^k = m \cdot 1 \equiv m \mod n$$
Therefore, 
$$m^{ed} \equiv m \mod n$$
NOTE: This only applies if $\gcd(m,n) = 1$ (as required by Euler's Theorem. There are ways to ensure this in practice.
#### Choose Encryption Exponent $e$
Choose a number $e$ s.t.:
- $1 < e < \phi(n)$
- $\gcd(e, \phi(n)) = 1$
$e$ will be the exponent in the encryption function $c = m^e \mod n$.
Therefore, it must be invertible $\mod \phi(n)$, so that decryption is possible.
#### Compute Decryption Exponent $d$
Solve for $d$ s.t.:
$$e \cdot d \equiv 1 \mod \phi(n)$$
This means that
$$d = e^{-1} \mod \phi(n)$$
$d$ basically undoes the encryption.
We use Extended EA to compute this $d$.
### Encryption
Given a plaintext message $m \in \mathbb{Z}$, we compute:
$$c = m^e \mod n$$
This works since we are applying a transformation to $m$ that is:
- easy to compute (fast modular exponentiation)
- hard to reverse without $d$ (computing $d$ requires factoring $n$, which is computationally infeasible if $n$ is large)
	- Why? EXPLORE THIS
### Decryption
As shown above, raising the ciphertext by the $d$ private key mod n returns back the original message $m$.
### Notes
1. $\gcd(m,n) = 1$ matters:
	- Euler's Theorem requires it
	- In practice, padding schemes ensure messages satisfy this.
2. What if $m \geq n$?
	- We must ensure $m < n$. In real systems, messages are often broke into blocks smaller than $n$.
3. String encoding
	- RSA doesn't encrypt raw strings, so messages are converted to integers via encoding (ex. ASCII)

## Square-and-Multiply (Binary Exponentiation) Algorithm
We often want to compute:
$$b^e \mod n$$
A naive approach is to compute:
$$b^e = b\cdot b \cdots b \mod n$$
This takes $O(e)$ multiplications, which is infeasible where $e$ is very large. 

Instead of this, we use **binary exponentiation**.
1. Convert exponent to binary
$$e = (e_k e_{k-1} \dots e_0)$$
2. For the first 1, just list the number
3. For each subsequent 0, square the current value
4. For each subsequent 1, square the current value and multiply by the base
Example: $3^5$
- $b = 3$, $e = 5$
- $e = 5 = 101$ (binary) 
- 1: first one lists the number: 3
- 0: zero does square: $(3)^2$
- 1: one does square and multiply: $((3)^2)^2 \cdot 3$
This algorithm only requires $O$($log$ e) operations.


